examples/dev/sw/working/0.1/ILScript.sml
@@ -1,10 +1,20 @@
-(*
-app load ["pred_setSimps","pred_setTheory","whileTheory","finite_mapTheory","rich_listTheory"];
+(* interactive use:
+
+quietdec := true;
+loadPath := (concat Globals.HOLDIR "/examples/dev/sw") :: !loadPath;
+
+app load ["pred_setSimps", "pred_setTheory",
+     "arithmeticTheory", "wordsTheory", "wordsLib", "pairTheory", "listTheory", "whileTheory", "finite_mapTheory", "preARMTheory", "ARMCompositionTheory",
+	  "relationTheory"];
+
+quietdec := false;
 *)
 
-open HolKernel Parse boolLib bossLib numLib pred_setSimps pred_setTheory
-     arithmeticTheory word32Theory pairTheory listTheory whileTheory finite_mapTheory preARMTheory ARMCompositionTheory;
 
+open HolKernel Parse boolLib bossLib numLib pred_setSimps pred_setTheory
+     arithmeticTheory wordsTheory wordsLib pairTheory listTheory whileTheory finite_mapTheory preARMTheory ARMCompositionTheory relationTheory;
+
+val _ = hide "B";
 (*---------------------------------------------------------------------------------*)
 (*---------------------------------------------------------------------------------*)
 
@@ -19,14 +29,11 @@ val set_ss = std_ss ++ SET_SPEC_ss ++ PRED_SET_ss;
 val _ = Hol_datatype ` 
     MREG = R0 | R1 | R2 | R3 | R4 | R5 | R6 | R7 | R8 | R9 | R10 | R11 | R12 | R13 | R14`;
 
-val _ = type_abbrev("MMEM", Type`:num # OFFSET`);      (* memory in ir *)
+val _ = type_abbrev("MMEM", Type`:MREG # OFFSET`);      (* memory in ir *)
 
 val _ = Hol_datatype `
     MEXP = MR of MREG          (* registers *)
-         | MC of DATA          (* constants *)
-         | MM of MMEM          (* memory    *)
-         | NA                  (* dummy     *)
-         | PR of MEXP # MEXP   (* pairs     *)
+         | MC of word4 => word8 (* constants *)
     `;
 
 val index_of_reg = Define `
@@ -44,8 +51,7 @@ val index_of_reg = Define `
     (index_of_reg R11 = 11) /\
     (index_of_reg R12 = 12) /\
     (index_of_reg R13 = 13) /\
-    (index_of_reg R14 = 14)
-`;
+    (index_of_reg R14 = 14)`;
 
 val from_reg_index_def = Define `
     from_reg_index i = 
@@ -91,13 +97,11 @@ val toREG_def = Define `
 
 val toMEM_def = Define `
     toMEM ((base,offset):MMEM) =
-       MEM (base,offset)`;        (* [base + offset] *)
+       preARM$MEM (index_of_reg base,offset)`;        (* [base + offset] *)
 
 val toEXP_def = Define `
     (toEXP (MR r) = toREG r) /\
-    (toEXP (MC c) = WCONST c) /\ 
-    (toEXP (MM m) = toMEM m)
-`;
+    (toEXP (MC shift c) = WCONST ((w2w c):word32 #>> (2*w2n shift)))`;
 
 (*---------------------------------------------------------------------------------*)
 (*      Semantics of the intermediate language                                     *)
@@ -107,21 +111,21 @@ val _ = Hol_datatype `
     DOPER = MLDR of MREG => MMEM |
            MSTR of MMEM => MREG |
            MMOV of MREG => MEXP |
-           MADD of MREG => MEXP => MEXP |
-           MSUB of MREG => MEXP => MEXP | 
-           MRSB of MREG => MEXP => MEXP |
-           MMUL of MREG => MEXP => MEXP |
-           MAND of MREG => MEXP => MEXP |
-           MORR of MREG => MEXP => MEXP |
-	   MEOR of MREG => MEXP => MEXP |
-	   MLSL of MREG => MEXP => MEXP |
-	   MLSR of MREG => MEXP => MEXP |
-	   MASR of MREG => MEXP => MEXP |
-	   MROR of MREG => MEXP => MEXP |
-           MPUSH of REGISTER => REGISTER list |
-	   MPOP of REGISTER => REGISTER list`;
+           MADD of MREG => MREG => MEXP |
+           MSUB of MREG => MREG => MEXP | 
+           MRSB of MREG => MREG => MEXP |
+           MMUL of MREG => MREG => MREG |
+           MAND of MREG => MREG => MEXP |
+           MORR of MREG => MREG => MEXP |
+     MEOR of MREG => MREG => MEXP |
+     MLSL of MREG => MREG => word5 |
+     MLSR of MREG => MREG => word5 |
+     MASR of MREG => MREG => word5 |
+     MROR of MREG => MREG => word5 |
+     MPUSH of num => num list |
+     MPOP of num => num list`;
 
-val _ = type_abbrev("CEXP", Type`:EXP # COND # EXP`);
+val _ = type_abbrev("CEXP", Type`:MREG # COND # MEXP`);
 
 val _ = Hol_datatype `CTL_STRUCTURE = 
     BLK of DOPER list |
@@ -142,14 +146,14 @@ val _ = Hol_datatype `CTL_STRUCTURE =
 val pushL_def =
   Define `pushL st baseR regL = 
    write (FST (FOLDL (\(st1,i) reg. (write st1 (MEM(baseR,NEG i)) (read st reg), i+1)) (st,0) (REVERSE (MAP REG regL))))
-         (REG baseR) (read st (REG baseR) - n2w (LENGTH regL))`;
+         (REG baseR) (read st (REG baseR) - n2w (4*LENGTH regL))`;
 
 (* Pop into multiple registers from the stack with writing-back to the sp   *)
  
 val popL_def =
   Define `popL st baseR regL = 
    write (FST (FOLDL (\(st1,i) reg. (write st1 reg (read st (MEM(baseR, POS(i+1)))), i+1)) (st,0) (MAP REG regL)))
-         (REG baseR) (read st (REG baseR) + n2w (LENGTH regL))`;
+         (REG baseR) (read st (REG baseR) + n2w (4*LENGTH regL))`;
 
 (*---------------------------------------------------------------------------------*)
 (*      Decode assignment statement                                                *)
@@ -163,27 +167,27 @@ val mdecode_def = Define `
   (mdecode st (MMOV dst src) =
       write st (toREG dst) (read st (toEXP src))) /\
   (mdecode st (MADD dst src1 src2) =
-      write st (toREG dst) (read st (toEXP src1) + read st (toEXP src2))) /\
+      write st (toREG dst) (read st (toREG src1) + read st (toEXP src2))) /\
   (mdecode st (MSUB dst src1 src2) =
-      write st (toREG dst) (read st (toEXP src1) - read st (toEXP src2))) /\
+      write st (toREG dst) (read st (toREG src1) - read st (toEXP src2))) /\
   (mdecode st (MRSB dst src1 src2) =
-      write st (toREG dst) (read st (toEXP src2) - read st (toEXP src1))) /\
-  (mdecode st (MMUL dst src1 src2) =
-      write st (toREG dst) (read st (toEXP src1) * read st (toEXP src2))) /\
+      write st (toREG dst) (read st (toEXP src2) - read st (toREG src1))) /\
+  (mdecode st (MMUL dst src1 src2_reg) =
+      write st (toREG dst) (read st (toREG src1) * read st (toREG src2_reg))) /\
   (mdecode st (MAND dst src1 src2) =
-      write st (toREG dst) (read st (toEXP src1) & read st (toEXP src2))) /\
+      write st (toREG dst) (read st (toREG src1) && read st (toEXP src2))) /\
   (mdecode st (MORR dst src1 src2) =
-      write st (toREG dst) (read st (toEXP src1) | read st (toEXP src2))) /\
+      write st (toREG dst) (read st (toREG src1) !! read st (toEXP src2))) /\
   (mdecode st (MEOR dst src1 src2) =
-      write st (toREG dst) (read st (toEXP src1) # read st (toEXP src2))) /\
-  (mdecode st (MLSL dst src1 src2) =
-      write st (toREG dst) (read st (toEXP src1) << w2n (read st (toEXP src2)))) /\
-  (mdecode st (MLSR dst src1 src2) =
-      write st (toREG dst) (read st (toEXP src1) >>> w2n (read st (toEXP src2)))) /\  
-  (mdecode st (MASR dst src1 src2) =
-      write st (toREG dst) (read st (toEXP src1) >> w2n (read st (toEXP src2)))) /\
-  (mdecode st (MROR dst src1 src2) =
-      write st (toREG dst) (read st (toEXP src1) #>> w2n (read st (toEXP src2)))) /\
+      write st (toREG dst) (read st (toREG src1) ?? read st (toEXP src2))) /\
+  (mdecode st (MLSL dst src2_reg src2_num) =
+      write st (toREG dst) (read st (toREG src2_reg) << w2n src2_num)) /\
+  (mdecode st (MLSR dst src2_reg src2_num) =
+      write st (toREG dst) (read st (toREG src2_reg) >>> w2n src2_num)) /\  
+  (mdecode st (MASR dst src2_reg src2_num) =
+      write st (toREG dst) (read st (toREG src2_reg) >> w2n src2_num)) /\
+  (mdecode st (MROR dst src2_reg src2_num) =
+      write st (toREG dst) (read st (toREG src2_reg) #>> w2n src2_num)) /\
   (mdecode st (MPUSH dst' srcL) =
       pushL st dst' srcL) /\
   (mdecode st (MPOP dst' srcL) =
@@ -192,22 +196,29 @@ val mdecode_def = Define `
 
 val translate_assignment_def = Define `
     (translate_assignment (MMOV dst src) = ((MOV,NONE,F),SOME (toREG dst), [toEXP src], NONE):INST) /\
-    (translate_assignment (MADD dst src1 src2) = ((ADD,NONE,F),SOME (toREG dst), [toEXP src1; toEXP src2], NONE):INST) /\
-    (translate_assignment (MSUB dst src1 src2) = ((SUB,NONE,F),SOME (toREG dst), [toEXP src1; toEXP src2], NONE):INST) /\
-    (translate_assignment (MRSB dst src1 src2) = ((RSB,NONE,F),SOME (toREG dst), [toEXP src1; toEXP src2], NONE):INST) /\
-    (translate_assignment (MMUL dst src1 src2) = ((MUL,NONE,F),SOME (toREG dst), [toEXP src1; toEXP src2], NONE):INST) /\
-    (translate_assignment (MAND dst src1 src2) = ((AND,NONE,F),SOME (toREG dst), [toEXP src1; toEXP src2], NONE):INST) /\
-    (translate_assignment (MORR dst src1 src2) = ((ORR,NONE,F),SOME (toREG dst), [toEXP src1; toEXP src2], NONE):INST) /\
-    (translate_assignment (MEOR dst src1 src2) = ((EOR,NONE,F),SOME (toREG dst), [toEXP src1; toEXP src2], NONE):INST) /\
-    (translate_assignment (MLSL dst src1 src2) = ((LSL,NONE,F),SOME (toREG dst), [toEXP src1; toEXP src2], NONE):INST) /\
-    (translate_assignment (MLSR dst src1 src2) = ((LSR,NONE,F),SOME (toREG dst), [toEXP src1; toEXP src2], NONE):INST) /\
-    (translate_assignment (MASR dst src1 src2) = ((ASR,NONE,F),SOME (toREG dst), [toEXP src1; toEXP src2], NONE):INST) /\
-    (translate_assignment (MROR dst src1 src2) = ((ROR,NONE,F),SOME (toREG dst), [toEXP src1; toEXP src2], NONE):INST) /\
+    (translate_assignment (MADD dst src1 src2) = ((ADD,NONE,F),SOME (toREG dst), [toREG src1; toEXP src2], NONE):INST) /\
+    (translate_assignment (MSUB dst src1 src2) = ((SUB,NONE,F),SOME (toREG dst), [toREG src1; toEXP src2], NONE):INST) /\
+    (translate_assignment (MRSB dst src1 src2) = ((RSB,NONE,F),SOME (toREG dst), [toREG src1; toEXP src2], NONE):INST) /\
+    (translate_assignment (MMUL dst src1 src2_reg) = ((MUL,NONE,F),SOME (toREG dst), [toREG src1; toREG src2_reg], NONE):INST) /\
+    (translate_assignment (MAND dst src1 src2) = ((AND,NONE,F),SOME (toREG dst), [toREG src1; toEXP src2], NONE):INST) /\
+    (translate_assignment (MORR dst src1 src2) = ((ORR,NONE,F),SOME (toREG dst), [toREG src1; toEXP src2], NONE):INST) /\
+    (translate_assignment (MEOR dst src1 src2) = ((EOR,NONE,F),SOME (toREG dst), [toREG src1; toEXP src2], NONE):INST) /\
+    (translate_assignment (MLSL dst src2_reg src2_num) = ((LSL,NONE,F),SOME (toREG dst), [toREG src2_reg; WCONST (w2w src2_num)], NONE):INST) /\
+    (translate_assignment (MLSR dst src2_reg src2_num) = ((LSR,NONE,F),SOME (toREG dst), [toREG src2_reg; WCONST (w2w src2_num)], NONE):INST) /\
+    (translate_assignment (MASR dst src2_reg src2_num) = ((ASR,NONE,F),SOME (toREG dst), [toREG src2_reg; WCONST (w2w src2_num)], NONE):INST) /\
+    (translate_assignment (MROR dst src2_reg src2_num) = ((ROR,NONE,F),SOME (toREG dst), [toREG src2_reg; WCONST (w2w src2_num)], NONE):INST) /\
     (!dst src.translate_assignment (MLDR dst src) = ((LDR,NONE,F),SOME (toREG dst), [toMEM src], NONE):INST) /\
     (!dst src.translate_assignment (MSTR dst src) = ((STR,NONE,F),SOME (toREG src), [toMEM dst], NONE):INST) /\
     (!dst srcL.translate_assignment (MPUSH dst srcL) = ((STMFD,NONE,F),SOME (WREG dst), MAP REG srcL, NONE):INST) /\
     (!dst srcL.translate_assignment (MPOP dst srcL) = ((LDMFD,NONE,F),SOME (WREG dst), MAP REG srcL, NONE):INST)
     `;
+
+val translate_condition_def = Define `
+  translate_condition (r, c, e) =
+    (toREG r, c, toEXP e)`
+
+val eval_il_cond_def = Define `
+  eval_il_cond cond = eval_cond (translate_condition cond)`;
 
 
 val TRANSLATE_ASSIGMENT_CORRECT = Q.store_thm
@@ -217,9 +228,8 @@ val TRANSLATE_ASSIGMENT_CORRECT = Q.store_thm
      SIMP_TAC std_ss [FORALL_DSTATE] THEN
      Cases_on `stm` THEN
      RW_TAC list_ss [translate_assignment_def, decode_cond_thm, decode_op_thm, write_thm,  mdecode_def] THEN
-     RW_TAC list_ss [pushL_def, popL_def]
+     RW_TAC list_ss [pushL_def, popL_def, read_thm, w2n_w2w, dimindex_5, dimindex_32]
   );
-
 
 val TRANSLATE_ASSIGMENT_CORRECT_2 = Q.store_thm
   ("TRANSLATE_ASSIGMENT_CORRECT_2",
@@ -228,6 +238,7 @@ val TRANSLATE_ASSIGMENT_CORRECT_2 = Q.store_thm
      RW_TAC std_ss [] THEN
      METIS_TAC [ABS_PAIR_THM,FST,SND,TRANSLATE_ASSIGMENT_CORRECT]
   );
+
 
 (*---------------------------------------------------------------------------------*)
 (*      Decode from intermedia language to low level language                      *)
@@ -239,9 +250,9 @@ val translate_def = Define `
     (translate (SC S1 S2) = 
          mk_SC (translate S1) (translate S2)) /\
     (translate (CJ cond Strue Sfalse) = 
-	 mk_CJ cond (translate Strue) (translate Sfalse)) /\
+	 mk_CJ (translate_condition cond) (translate Strue) (translate Sfalse)) /\
     (translate (TR cond Sbody) = 
-         mk_TR cond (translate Sbody))
+         mk_TR (translate_condition cond) (translate Sbody))
   `;
 
 (*---------------------------------------------------------------------------------*)
@@ -255,8 +266,51 @@ val run_arm_def = Define `
 val run_ir_def = Define `
       run_ir ir st = get_st (run_arm (translate ir) ((0,0w,st),{}))`;
 
+
 val WELL_FORMED_def = Define `
-      WELL_FORMED ir = well_formed (translate ir)`;
+      (WELL_FORMED (BLK stmL) = well_formed (translate (BLK stmL))) /\
+      (WELL_FORMED (SC S1 S2) = well_formed (translate (SC S1 S2)) /\
+                                WELL_FORMED S1 /\ WELL_FORMED S2) /\
+      (WELL_FORMED (CJ cond S1 S2) = well_formed (translate (CJ cond S1 S2)) /\
+                                WELL_FORMED S1 /\ WELL_FORMED S2) /\
+      (WELL_FORMED (TR cond S1) = well_formed (translate (TR cond S1)) /\
+                                WELL_FORMED S1 /\
+                                WF_TR (translate_condition cond, translate S1))`;
+
+
+val WELL_FORMED_SUB_def = Define `
+      (WELL_FORMED_SUB (BLK stmL) = T) /\
+      (WELL_FORMED_SUB (SC S1 S2) = WELL_FORMED S1 /\ WELL_FORMED S2) /\
+      (WELL_FORMED_SUB (CJ cond S1 S2) = WELL_FORMED S1 /\ WELL_FORMED S2) /\
+      (WELL_FORMED_SUB (TR cond S1) = WELL_FORMED S1 /\ WF_TR (translate_condition cond, translate S1))`;
+
+val WELL_FORMED_SUB_thm = store_thm ("WELL_FORMED_SUB_thm",
+    ``!ir. WELL_FORMED ir = (WELL_FORMED_SUB ir /\ well_formed (translate ir))``,
+
+    Cases_on `ir` THEN
+    REWRITE_TAC [WELL_FORMED_def, WELL_FORMED_SUB_def] THEN
+    PROVE_TAC[]);
+
+
+val CHANGED_def = Define `CHANGED s ir =
+	!st st'. (st' = run_ir ir st) ==> (
+		!r. ~(MEM r s) ==> (read st (toREG r) = read st' (toREG r))
+	)`
+
+val UNCHANGED_def = Define `UNCHANGED s ir =
+	!st st'. (st' = run_ir ir st) ==> (
+		!r. (MEM r s) ==> (read st (toREG r) = read st' (toREG r))
+	)`
+
+
+val UNCHANGED_THM = store_thm ("UNCHANGED_THM",
+
+	``!s ir.
+		UNCHANGED s ir =
+		EVERY (\r. !reg mem. (read (reg,mem) (toREG r) = read (run_ir ir (reg,mem)) (toREG r))) s``,
+
+	SIMP_TAC std_ss [EVERY_MEM, UNCHANGED_def, ELIM_PFORALL] THEN
+	METIS_TAC[pairTheory.PAIR])
 
 (*---------------------------------------------------------------------------------*)
 (*      Hoare Rules for IR                                                         *) 
@@ -270,7 +324,7 @@ val HOARE_SC_IR = Q.store_thm (
            (!st. R st ==> T (run_ir ir2 st)) /\ (!st. Q st ==> R st) ==>
              !st. P st ==>
                   T (run_ir (SC ir1 ir2) st)`,
-   RW_TAC std_ss [WELL_FORMED_def, run_ir_def, translate_def, run_arm_def, eval_fl_def] THEN 
+   RW_TAC std_ss [WELL_FORMED_SUB_thm, run_ir_def, translate_def, run_arm_def, eval_fl_def] THEN 
    IMP_RES_TAC (SIMP_RULE std_ss [eval_fl_def, uploadCode_def]  HOARE_SC_FLAT)
   );
 
@@ -281,9 +335,9 @@ val HOARE_CJ_IR = Q.store_thm (
            (!st. P st ==> Q (run_ir ir_t st)) /\
            (!st. P st ==> R (run_ir ir_f st)) ==>
              !st. P st ==>
-                if eval_cond cond st then Q (run_ir (CJ cond ir_t ir_f) st)
+                if eval_il_cond cond st then Q (run_ir (CJ cond ir_t ir_f) st)
                     else R (run_ir (CJ cond ir_t ir_f) st)`,
-   RW_TAC std_ss [WELL_FORMED_def, run_ir_def, translate_def, run_arm_def, eval_fl_def] THEN
+   RW_TAC std_ss [WELL_FORMED_SUB_thm, run_ir_def, translate_def, run_arm_def, eval_fl_def, eval_il_cond_def] THEN
    IMP_RES_TAC (SIMP_RULE std_ss [eval_fl_def, uploadCode_def] HOARE_CJ_FLAT) THEN
    METIS_TAC []
   );
@@ -291,11 +345,11 @@ val HOARE_CJ_IR = Q.store_thm (
 val HOARE_TR_IR = Q.store_thm (
    "HOARE_TR_IR",
    `!cond ir P.
-       WELL_FORMED ir /\  WF_TR (cond, translate ir) /\
+       WELL_FORMED ir /\  WF_TR (translate_condition cond, translate ir) /\
          (!st. P st ==> P (run_ir ir st)) ==>
             !st. P st ==> P (run_ir (TR cond ir) st) /\ 
-                 eval_cond cond (run_ir (TR cond ir) st)`,
-   RW_TAC std_ss [WELL_FORMED_def, run_ir_def, translate_def, run_arm_def, eval_fl_def] THEN
+                 eval_il_cond cond (run_ir (TR cond ir) st)`,
+   RW_TAC std_ss [WELL_FORMED_SUB_thm, run_ir_def, translate_def, run_arm_def, eval_fl_def, eval_il_cond_def] THEN
    METIS_TAC [SIMP_RULE std_ss [eval_fl_def, uploadCode_def] HOARE_TR_FLAT]
   );
 
@@ -327,11 +381,11 @@ val STATEMENT_IS_WELL_FORMED = Q.store_thm (
         Cases_on `stm` THEN
             (fn g => 
                (SIMP_TAC list_ss [get_st_def, Once RUNTO_ADVANCE, SIMP_RULE std_ss [] (Q.SPEC `(pos0,cpsr0,regs,mem):STATE` 
-			  (INST_TYPE [alpha |-> Type `:word32 # (num |-> word32) # (num |-> word32)`] UPLOAD_LEM_2)), 
+			  (INST_TYPE [alpha |-> Type `:word32 # (word4 |-> word32) # (word30 |-> word32)`] UPLOAD_LEM_2)), 
                          TRANSLATE_ASSIGMENT_CORRECT_2, SUC_ONE_ADD] THEN
                 RW_TAC std_ss [Once RUNTO_ADVANCE] THEN
                 SIMP_TAC list_ss [get_st_def, Once RUNTO_ADVANCE, SIMP_RULE std_ss [] (Q.SPEC `(pos1,cpsr1,regs,mem):STATE` 
-			  (INST_TYPE [alpha |-> Type `:word32 # (num |-> word32) # (num |-> word32)`] UPLOAD_LEM_2)), 
+			  (INST_TYPE [alpha |-> Type `:word32 # (word4 |-> word32) # (word30 |-> word32)`] UPLOAD_LEM_2)), 
                          TRANSLATE_ASSIGMENT_CORRECT_2, SUC_ONE_ADD] THEN
                 RW_TAC std_ss [Once RUNTO_ADVANCE]) g
             )
@@ -355,28 +409,35 @@ val BLOCK_IS_WELL_FORMED = Q.store_thm (
 
 val IR_SC_IS_WELL_FORMED = Q.store_thm (
    "IR_SC_IS_WELL_FORMED",
-   `!ir1 ir2. WELL_FORMED ir1 /\ WELL_FORMED ir2 ==>
-        WELL_FORMED (SC ir1 ir2)`,
-    RW_TAC std_ss [WELL_FORMED_def, translate_def] THEN
-    IMP_RES_TAC (SC_IS_WELL_FORMED)
+   `!ir1 ir2. WELL_FORMED ir1 /\ WELL_FORMED ir2 = WELL_FORMED (SC ir1 ir2)`,
+    RW_TAC std_ss [WELL_FORMED_SUB_thm, WELL_FORMED_SUB_def, translate_def] THEN
+    PROVE_TAC [SC_IS_WELL_FORMED]
    );
 
 val IR_CJ_IS_WELL_FORMED = Q.store_thm (
    "IR_CJ_IS_WELL_FORMED",
-   `!cond ir_t ir_f. WELL_FORMED ir_t /\ WELL_FORMED ir_f ==>
+   `!cond ir_t ir_f. WELL_FORMED ir_t /\ WELL_FORMED ir_f =
         WELL_FORMED (CJ cond ir_t ir_f)`,
-    RW_TAC std_ss [WELL_FORMED_def, translate_def] THEN
-    IMP_RES_TAC (CJ_IS_WELL_FORMED) THEN
-    METIS_TAC []
+    RW_TAC std_ss [WELL_FORMED_SUB_thm, WELL_FORMED_SUB_def, translate_def] THEN
+    PROVE_TAC [CJ_IS_WELL_FORMED]
    );
 
 val IR_TR_IS_WELL_FORMED = Q.store_thm (
    "IR_TR_IS_WELL_FORMED",
-   `!ir cond. WELL_FORMED ir /\ WF_TR (cond, translate ir) ==>
+   `!ir cond. WELL_FORMED ir /\ WF_TR (translate_condition cond, translate ir) =
         WELL_FORMED (TR cond ir)`,
-    RW_TAC std_ss [WELL_FORMED_def, translate_def] THEN
-    IMP_RES_TAC (TR_IS_WELL_FORMED)
+    RW_TAC std_ss [WELL_FORMED_SUB_thm, WELL_FORMED_SUB_def, translate_def] THEN
+    PROVE_TAC [TR_IS_WELL_FORMED]
    );
+
+val WELL_FORMED_thm = store_thm ("WELL_FORMED_thm",
+    ``(WELL_FORMED (BLK stmL) = T) /\
+      (WELL_FORMED (SC S1 S2) = WELL_FORMED S1 /\ WELL_FORMED S2) /\
+      (WELL_FORMED (CJ cond S1 S2) = WELL_FORMED S1 /\ WELL_FORMED S2) /\
+      (WELL_FORMED (TR cond S1) = WELL_FORMED S1 /\ WF_TR (translate_condition cond, translate S1))``,
+
+      SIMP_TAC std_ss [BLOCK_IS_WELL_FORMED, IR_SC_IS_WELL_FORMED, IR_CJ_IS_WELL_FORMED, IR_TR_IS_WELL_FORMED]);
+
 
 (*---------------------------------------------------------------------------------*)
 (*      Semantics of IR                                                            *) 
@@ -418,7 +479,7 @@ val IR_SEMANTICS_CJ = Q.store_thm (
    "IR_SEMANTICS_CJ",
    ` WELL_FORMED ir_t /\ WELL_FORMED ir_f ==>
      (run_ir (CJ cond ir_t ir_f) st = 
-          if eval_cond cond st then run_ir ir_t st
+          if eval_il_cond cond st then run_ir ir_t st
           else run_ir ir_f st)`,
    RW_TAC std_ss [] THEN
    METIS_TAC [SIMP_RULE std_ss [] (Q.SPECL [`cond`, `ir_t`, `ir_f`, `\st'. st' = st`, `\st'. st' = run_ir ir_t st`, 
@@ -428,24 +489,24 @@ val IR_SEMANTICS_CJ = Q.store_thm (
 
 val IR_SEMANTICS_TR = Q.store_thm (
    "IR_SEMANTICS_TR",
-     `WELL_FORMED ir /\ WF_TR (cond,translate ir) ==>
+     `WELL_FORMED ir /\ WF_TR (translate_condition cond,translate ir) ==>
       (run_ir (TR cond ir) st =
-         WHILE (\st'.~eval_cond cond st') (run_ir ir) st)`,
+         WHILE (\st'.~eval_il_cond cond st') (run_ir ir) st)`,
 
-    RW_TAC std_ss [WELL_FORMED_def, run_ir_def, run_arm_def, translate_def] THEN
+    RW_TAC std_ss [WELL_FORMED_SUB_thm, run_ir_def, run_arm_def, translate_def, eval_il_cond_def] THEN
     Q.ABBREV_TAC `arm = translate ir` THEN
-    IMP_RES_TAC (SIMP_RULE set_ss [] (Q.SPECL [`cond`,`arm`,`(\i. ARB)`,`(0,0w,st):STATE`,`{}`] UNROLL_TR_LEM)) THEN
+    IMP_RES_TAC (SIMP_RULE set_ss [] (Q.SPECL [`translate_condition cond`,`arm`,`(\i. ARB)`,`(0,0w,st):STATE`,`{}`] UNROLL_TR_LEM)) THEN
     POP_ASSUM (ASSUME_TAC o Q.SPEC `st`) THEN
     FULL_SIMP_TAC std_ss [FUNPOW,get_st_def] THEN
     NTAC 2 (POP_ASSUM (K ALL_TAC)) THEN
-    Induct_on `loopNum cond arm (\i.ARB) ((0,0w,st),{})` THENL [
+    Induct_on `loopNum (translate_condition cond) arm (\i.ARB) ((0,0w,st),{})` THENL [
         REWRITE_TAC [Once EQ_SYM_EQ] THEN RW_TAC std_ss [FUNPOW,get_st_def] THEN
             IMP_RES_TAC LOOPNUM_BASIC THEN
             FULL_SIMP_TAC arith_ss [Once WHILE, get_st_def],
 
         REWRITE_TAC [Once EQ_SYM_EQ] THEN RW_TAC std_ss [FUNPOW] THEN
             IMP_RES_TAC LOOPNUM_INDUCTIVE THEN
-            `v = loopNum cond arm (\i.ARB) ((0,0w,SND (SND (FST (runTo (upload arm (\i.ARB) 0) (LENGTH arm) ((0,0w,st),{}))))),{})` by
+            `v = loopNum (translate_condition cond) arm (\i.ARB) ((0,0w,SND (SND (FST (runTo (upload arm (\i.ARB) 0) (LENGTH arm) ((0,0w,st),{}))))),{})` by
             METIS_TAC [ABS_PAIR_THM,DECIDE (Term`!x.0+x=x`),LOOPNUM_INDEPENDENT_OF_CPSR_PCS, get_st_def, FST, SND, DSTATE_IRRELEVANT_PCS, 
 		well_formed_def] THEN
             RES_TAC THEN Q.PAT_ASSUM `v = x` (ASSUME_TAC o GSYM) THEN FULL_SIMP_TAC std_ss [] THEN POP_ASSUM (K ALL_TAC) THEN
@@ -460,18 +521,136 @@ val IR_SEMANTICS_TR = Q.store_thm (
   );
 
 
+val IR_SEMANTICS_EMBEDDED_THM = Q.store_thm (
+   "IR_SEMANTICS_EMBEDDED_THM",
+		`!ir s. well_formed (translate ir) ==>
+				(?pc cpsr pcS. 	  
+				(run_arm (translate ir) s = ((pc, cpsr, run_ir ir (SND(SND(FST s)))), pcS)))`,
+
+		SIMP_TAC std_ss [run_ir_def, well_formed_def] THEN
+		REPEAT STRIP_TAC THEN
+		`?pc cpsr st pcS. (s = ((pc,cpsr,st),pcS))` by METIS_TAC[PAIR, FST, SND] THEN
+		ASM_REWRITE_TAC [run_arm_def] THEN
+		Q.ABBREV_TAC `arm = (translate ir)` THEN
+		`get_st (runTo (upload arm (\i. ARB) 0) (0 + LENGTH arm) ((0,0w,st),{})) =
+		 get_st (runTo (upload arm (\i. ARB) pc) (pc + LENGTH arm) ((pc,cpsr,st),pcS))`
+			 by METIS_TAC[status_independent_def, DSTATE_IRRELEVANT_PCS, FST] THEN
+		ASM_SIMP_TAC std_ss [get_st_def] THEN 
+		METIS_TAC[PAIR, FST, SND]);
+
+
+
+
+val WF_ir_TR_def =  Define `
+	WF_ir_TR (cond, ir) =
+		WF_Loop ((eval_il_cond cond),
+              (run_ir ir))`;
+
+
+val WF_ir_TR_thm = Q.store_thm (
+   "WF_ir_TR_thm",
+	  `!cond ir. WELL_FORMED ir ==>
+		(WF_ir_TR (cond, ir) = WF_TR (translate_condition cond, translate ir))`,
+
+SIMP_TAC std_ss [WF_ir_TR_def, WF_TR_def, WF_Loop_def, eval_il_cond_def, WELL_FORMED_SUB_thm] THEN
+REPEAT STRIP_TAC THEN EQ_TAC THEN REPEAT STRIP_TAC THENL [
+	Q_TAC EXISTS_TAC `inv_image R get_st` THEN
+	ASM_SIMP_TAC std_ss [WF_inv_image] THEN
+	GEN_TAC THEN
+	`?pc' cpsr' pcS'. run_arm (translate ir) s =
+		((pc',cpsr',run_ir ir (SND (SND (FST s)))),pcS')` by 
+		METIS_TAC[IR_SEMANTICS_EMBEDDED_THM] THEN
+	`?pc cpsr st pcS. (s = ((pc,cpsr,st),pcS))` by METIS_TAC[PAIR, FST, SND] THEN
+	`runTo (upload (translate ir) iB pc) (pc + LENGTH (translate ir))
+				((pc,cpsr,st),pcS) =
+	run_arm (translate ir) ((pc,cpsr,st),pcS)` by ALL_TAC THEN1 (
+		SIMP_TAC std_ss [run_arm_def] THEN
+		METIS_TAC[WELL_FORMED_INSTB, FST]
+	) THEN
+	FULL_SIMP_TAC std_ss [relationTheory.inv_image_def, get_st_def],
+
+
+	
+	FULL_SIMP_TAC std_ss [FORALL_PROD] THEN
+	`!iB pc cpsr st pcS. runTo (upload (translate ir) iB pc) (pc + LENGTH (translate ir))
+				((pc,cpsr,st),pcS) =
+	run_arm (translate ir) ((pc,cpsr,st),pcS)` by ALL_TAC THEN1 (
+		SIMP_TAC std_ss [run_arm_def] THEN
+		METIS_TAC[WELL_FORMED_INSTB, FST]
+	) THEN
+	FULL_SIMP_TAC std_ss [] THEN
+	POP_ASSUM (fn thm => ALL_TAC) THEN
+
+	`?Q. Q = \st st'. !s'. 
+	   let s = (run_arm (translate ir) s') in
+		(((get_st s' = st')) ==> ((get_st s = st) /\
+	     R s s'))` by METIS_TAC[] THEN
+	Q_TAC EXISTS_TAC `Q` THEN
+	REPEAT STRIP_TAC THENL [
+		FULL_SIMP_TAC std_ss [WF_DEF, LET_THM] THEN
+		REPEAT STRIP_TAC THEN
+		`?B'. B' = (\s. B (get_st s))` by METIS_TAC[] THEN
+		Q.PAT_ASSUM `!B. (?w. B w) ==> X` (fn thm => Q_TAC 
+			(fn t => (ASSUME_TAC (SPEC t thm))) `B'`) THEN
+		Q.PAT_UNDISCH_TAC `X` THEN
+		SIMP_TAC std_ss [GSYM LEFT_FORALL_IMP_THM,
+			GSYM LEFT_EXISTS_IMP_THM] THEN
+
+		`?w. B (get_st w)` by METIS_TAC[get_st_def, PAIR, FST, SND] THEN
+		Q_TAC EXISTS_TAC `w'` THEN
+		ASM_SIMP_TAC std_ss [] THEN
+		REPEAT STRIP_TAC THEN
+		Q_TAC EXISTS_TAC `get_st min` THEN
+		ASM_SIMP_TAC std_ss [] THEN
+		GEN_TAC THEN
+		Q_TAC EXISTS_TAC `min` THEN
+		SIMP_TAC std_ss [] THEN
+	   METIS_TAC[],
+
+
+		FULL_SIMP_TAC std_ss [LET_THM, get_st_def, run_ir_def] THEN
+		GEN_TAC THEN
+		`?pc cpsr st pcS. (s' = ((pc,cpsr,st),pcS))` by METIS_TAC[PAIR, FST, SND] THEN
+		ASM_SIMP_TAC std_ss [] THEN
+		FULL_SIMP_TAC std_ss [GSYM get_st_def, run_arm_def,  well_formed_def] THEN
+
+		`(LENGTH (translate ir)) = 0 + (LENGTH (translate ir))` by DECIDE_TAC THEN
+		METIS_TAC[status_independent_def, DSTATE_IRRELEVANT_PCS, FST]
+	]
+]);
+
+
+
+val IR_SEMANTICS_TR___FUNPOW = Q.store_thm (
+   "IR_SEMANTICS_TR___FUNPOW",
+     `WELL_FORMED ir /\ WF_TR (translate_condition cond,translate ir) ==>
+      (run_ir (TR cond ir) st =
+        FUNPOW (run_ir ir) (shortest (eval_il_cond cond) (run_ir ir) st) st)`,
+
+
+	SIMP_TAC std_ss [IR_SEMANTICS_TR] THEN
+	REPEAT STRIP_TAC THEN
+	`(\st'. ~eval_il_cond cond st') = $~ o (eval_il_cond cond)` by SIMP_TAC std_ss [combinTheory.o_DEF] THEN
+	ASM_SIMP_TAC std_ss [] THEN
+	MATCH_MP_TAC ARMCompositionTheory.UNROLL_LOOP THEN
+	METIS_TAC[WF_ir_TR_thm, WF_ir_TR_def]);
+
+
+
+
 val SEMANTICS_OF_IR = Q.store_thm (
    "SEMANTICS_OF_IR",
-   ` WELL_FORMED ir1 /\ WELL_FORMED ir2 ==>
-     (run_ir (BLK (stm::stmL)) st =
+   `(run_ir (BLK []) st = st) /\
+    (run_ir (BLK (stm::stmL)) st =
           run_ir (BLK stmL) (mdecode st stm)) /\
-     (run_ir (BLK []) st = st) /\
-     (run_ir (SC ir1 ir2) st = run_ir ir2 (run_ir ir1 st)) /\
+    ((WELL_FORMED ir1 /\ WELL_FORMED ir2) ==>
+    (run_ir (SC ir1 ir2) st = run_ir ir2 (run_ir ir1 st))) /\
+    ((WELL_FORMED ir1 /\ WELL_FORMED ir2) ==>	 
      (run_ir (CJ cond ir1 ir2) st =
-           (if eval_cond cond st then run_ir ir1 st else run_ir ir2 st)) /\
-     ( WF_TR (cond,translate ir1) ==> 
+           (if eval_il_cond cond st then run_ir ir1 st else run_ir ir2 st))) /\
+     (( WELL_FORMED ir1 /\ WF_TR (translate_condition cond,translate ir1)) ==> 
        (run_ir (TR cond ir1) st =
-           WHILE (\st'. ~eval_cond cond st') (run_ir ir1) st))`,
+           WHILE (\st'. ~eval_il_cond cond st') (run_ir ir1) st))`,
    RW_TAC std_ss [IR_SEMANTICS_BLK, IR_SEMANTICS_CJ, IR_SEMANTICS_SC, IR_SEMANTICS_TR]
   );       
 
