examples/dev/sw/working/0.1/rulesScript.sml
@@ -1,6 +1,17 @@
+(* interactive use:
+
+quietdec := true;
+loadPath := (concat Globals.HOLDIR "/examples/dev/sw") :: !loadPath;
+
+app load ["numLib", "relationTheory", "arithmeticTheory", "preARMTheory", "pairTheory",
+     "pred_setSimps", "pred_setTheory", "listTheory", "rich_listTheory", "whileTheory", "ARMCompositionTheory", "ILTheory", "wordsTheory"];
+
+quietdec := false;
+*)
+
 
 open HolKernel Parse boolLib bossLib numLib relationTheory arithmeticTheory preARMTheory pairTheory
-     pred_setSimps pred_setTheory listTheory rich_listTheory whileTheory ARMCompositionTheory ILTheory;
+     pred_setSimps pred_setTheory listTheory rich_listTheory whileTheory ARMCompositionTheory ILTheory wordsTheory;
 
 
 val _ = new_theory "rules";
@@ -20,12 +31,19 @@ val _ = Globals.priming := NONE;
 (*---------------------------------------------------------------------------------*)
 (*      read from an data state                                                    *) 
 (*---------------------------------------------------------------------------------*)
+val _ = Hol_datatype `
+    REXP = RR of MREG          
+         | RM of MMEM          
+         | RC of DATA          
+         | PR of REXP # REXP
+    `;
+
 
 val mread_def = Define `
-    (mread st (MR r) = read st (toREG r)) /\
-    (mread st (MC c) = read st (WCONST c)) /\
-    (mread st (MM m) = read st (toMEM m))`;
-       
+     (mread st (RR r) = read st (toREG r)) /\
+     (mread st (RM m) = read st (toMEM m)) /\
+     (mread st (RC c) = c)`;
+
 val _ = add_rule {term_name = "mread", fixity = Suffix 60,
 		  pp_elements = [TOK "<", TM, TOK ">"],
                   paren_style = OnlyIfNecessary,
@@ -37,7 +55,7 @@ val _ = add_rule {term_name = "mread", fixity = Suffix 60,
 (*---------------------------------------------------------------------------------*)
 
 val proper_def = Define `
-    proper = (\(regs,mem):DSTATE. (regs ' 11 = 100w) /\ (regs ' 13 = 100w))`;
+    proper = (\(regs,mem):DSTATE. (regs ' 11w = 100w) /\ (regs ' 13w = 100w))`;
 
 
 (*---------------------------------------------------------------------------------*)
@@ -129,7 +147,7 @@ val BLK_RULE = Q.store_thm (
 val CJ_RULE = Q.store_thm (
    "CJ_RULE",
    `!P Q cond ir1 ir2 st. WELL_FORMED ir1 /\ WELL_FORMED ir2 /\
-      HSPEC (\st.eval_cond cond st /\ P st) ir1 Q /\ HSPEC (\st.~eval_cond cond st /\ P st) ir2 Q ==> 
+      HSPEC (\st.eval_il_cond cond st /\ P st) ir1 Q /\ HSPEC (\st.~eval_il_cond cond st /\ P st) ir2 Q ==> 
       HSPEC P (CJ cond ir1 ir2) Q`,
     RW_TAC std_ss [HSPEC_def] THEN 
     METIS_TAC [IR_SEMANTICS_CJ]
@@ -152,7 +170,7 @@ val CJ_RULE_2 = Q.store_thm (
 val TR_RULE = Q.store_thm (
    "TR_RULE",
    `!cond ir P Q.
-        WELL_FORMED ir /\  WF_TR (cond, translate ir) /\
+        WELL_FORMED ir /\  WF_TR (translate_condition cond, translate ir) /\
            HSPEC P ir P ==> HSPEC P (TR cond ir) P`,
    RW_TAC std_ss [HSPEC_def] THEN
    METIS_TAC [HOARE_TR_IR]
@@ -171,12 +189,12 @@ val WF_DEF_2 = Q.store_thm (
 val WF_TR_LEM_1 = Q.store_thm (
    "WF_TR_LEM_1",
    `!cond ir st. WELL_FORMED ir /\
-           WF (\st1 st0. ~eval_cond cond st0 /\ (st1 = run_ir ir st0)) ==>
-           WF_TR (cond,translate ir)`,
+           WF (\st1 st0. ~eval_il_cond cond st0 /\ (st1 = run_ir ir st0)) ==>
+           WF_TR (translate_condition cond,translate ir)`,
    
-   RW_TAC std_ss [WELL_FORMED_def, WF_TR_def, WF_Loop_def, run_ir_def, run_arm_def] THEN
+   RW_TAC std_ss [WELL_FORMED_SUB_thm, WF_TR_def, WF_Loop_def, run_ir_def, run_arm_def] THEN
    POP_ASSUM MP_TAC THEN Q.ABBREV_TAC `arm = translate ir` THEN STRIP_TAC THEN
-   Q.EXISTS_TAC `\s1 s0. if eval_cond cond (get_st s0) then F else (get_st s1 = get_st (runTo (upload arm (\i. ARB) (FST (FST s0))) 
+   Q.EXISTS_TAC `\s1 s0. if eval_il_cond cond (get_st s0) then F else (get_st s1 = get_st (runTo (upload arm (\i. ARB) (FST (FST s0))) 
              (FST (FST s0) + LENGTH (translate ir)) s0))` THEN
    STRIP_TAC THENL [
       FULL_SIMP_TAC std_ss [WF_DEF_2, GSYM RIGHT_FORALL_IMP_THM] THEN
@@ -193,7 +211,7 @@ val WF_TR_LEM_1 = Q.store_thm (
               METIS_TAC [well_formed_def, get_st_def, DSTATE_IRRELEVANT_PCS, status_independent_def, FST, DECIDE (Term `!x.0 + x = x`)] THEN
           METIS_TAC [FST,SND,get_st_def, ABS_PAIR_THM],
 
-      RW_TAC std_ss [get_st_def] THEN
+      RW_TAC std_ss [get_st_def, eval_il_cond_def] THEN
           METIS_TAC [WELL_FORMED_INSTB]
       ]
    );
@@ -201,9 +219,9 @@ val WF_TR_LEM_1 = Q.store_thm (
 val WF_TR_LEM_2 = Q.store_thm (
    "WF_TR_LEM_2",
     `!cond ir prj_f f cond_f.
-        (!st. cond_f (prj_f st) = eval_cond cond st) /\ (!st. prj_f (run_ir ir st) = f (prj_f st)) /\ 
+        (!st. cond_f (prj_f st) = eval_il_cond cond st) /\ (!st. prj_f (run_ir ir st) = f (prj_f st)) /\ 
         WF (\t1 t0. ~cond_f t0 /\ (t1 = f t0)) ==>
-           WF (\st1 st0. ~eval_cond cond st0 /\ (st1 = run_ir ir st0))`,
+           WF (\st1 st0. ~eval_il_cond cond st0 /\ (st1 = run_ir ir st0))`,
 
    RW_TAC std_ss [WF_DEF_2] THEN
    Q.PAT_ASSUM `!P.p` (ASSUME_TAC o Q.SPEC `\t:'a. ?y:DSTATE. (prj_f y = t) /\ P y`) THEN
@@ -230,10 +248,10 @@ val WF_TR_LEM_3 = Q.store_thm (
 val WF_TR_THM_1 = Q.store_thm (
    "WF_TR_THM_1",
     `!cond ir prj_f f cond_f pre_p.
-        (!st. cond_f (prj_f st) = eval_cond cond st) /\
+        (!st. cond_f (prj_f st) = eval_il_cond cond st) /\
         (!st. pre_p st ==> (prj_f (run_ir ir st) = f (prj_f st))) /\
         WF (\t1 t0. ~cond_f t0 /\ (t1 = f t0)) ==>
-           WF (\st1 st0. (pre_p st0) /\ ~(eval_cond cond st0) /\ (st1 = run_ir ir st0))`,
+           WF (\st1 st0. (pre_p st0) /\ ~(eval_il_cond cond st0) /\ (st1 = run_ir ir st0))`,
 
    RW_TAC std_ss [WF_DEF_2] THEN
    Q.PAT_ASSUM `!P.p` (ASSUME_TAC o Q.SPEC `\t:'a. ?y:DSTATE. (prj_f y = t) /\ P y`) THEN
@@ -315,7 +333,7 @@ val PRJ_CJ_RULE = Q.store_thm (
    `!cond ir_t ir_f pre_p post_p stk_f cond_f in_f f1 f2 out_f. 
      WELL_FORMED ir_t /\ WELL_FORMED ir_f /\
      PSPEC ir_t (pre_p,post_p) stk_f (in_f,f1,out_f) /\ 
-     PSPEC ir_f (pre_p, post_p) stk_f (in_f,f2,out_f) /\ (!st. cond_f (in_f st) = eval_cond cond st)
+     PSPEC ir_f (pre_p, post_p) stk_f (in_f,f2,out_f) /\ (!st. cond_f (in_f st) = eval_il_cond cond st)
         ==>
        PSPEC (CJ cond ir_t ir_f) (pre_p,post_p) stk_f (in_f, (\v.if cond_f v then f1 v else f2 v), out_f)`,
      
@@ -324,12 +342,11 @@ val PRJ_CJ_RULE = Q.store_thm (
    );
 
 (* Need the theorems in ARMCompositionTheory to prove the PROJ_TR_RULE *)
-
 val PRJ_TR_RULE = Q.store_thm (
    "PRJ_TR_RULE",
    `!cond ir pre_p stk_f cond_f prj_f f.
-        WELL_FORMED ir /\  WF (\st1 st0. ~eval_cond cond st0 /\ (st1 = run_ir ir st0)) /\
-        (!st. cond_f (prj_f st) = eval_cond cond st) /\ PSPEC ir (pre_p,pre_p) stk_f (prj_f,f,prj_f) ==> 
+        WELL_FORMED ir /\  WF (\st1 st0. ~eval_il_cond cond st0 /\ (st1 = run_ir ir st0)) /\
+        (!st. cond_f (prj_f st) = eval_il_cond cond st) /\ PSPEC ir (pre_p,pre_p) stk_f (prj_f,f,prj_f) ==> 
           PSPEC (TR cond ir) (pre_p,pre_p) stk_f (prj_f, WHILE ($~ o cond_f) f, prj_f)`,
 
     RW_TAC std_ss [PSPEC_def] THEN 
@@ -347,22 +364,22 @@ val PRJ_TR_RULE = Q.store_thm (
 
         IMP_RES_TAC (SIMP_RULE std_ss [PSPEC_def] PSPEC_CHARACTERISTIC) THEN
             Q.PAT_ASSUM `!v x.p` (K ALL_TAC) THEN
-            `WF_TR (cond,translate ir)` by METIS_TAC [WF_TR_LEM_1] THEN
-	    FULL_SIMP_TAC std_ss [WELL_FORMED_def, HSPEC_def, run_ir_def, run_arm_def, translate_def] THEN
+            `WF_TR (translate_condition cond,translate ir)` by METIS_TAC [WF_TR_LEM_1] THEN
+	    FULL_SIMP_TAC std_ss [WELL_FORMED_SUB_thm, HSPEC_def, run_ir_def, run_arm_def, translate_def, eval_il_cond_def] THEN
 	    Q.ABBREV_TAC `arm = translate ir` THEN
-	    IMP_RES_TAC (SIMP_RULE set_ss [] (Q.SPECL [`cond`,`arm`,`(\i. ARB)`,`(0,0w,st):STATE`,`{}`] 
+	    IMP_RES_TAC (SIMP_RULE set_ss [] (Q.SPECL [`translate_condition cond`,`arm`,`(\i. ARB)`,`(0,0w,st):STATE`,`{}`] 
                               ARMCompositionTheory.UNROLL_TR_LEM)) THEN
 	    POP_ASSUM (ASSUME_TAC o Q.SPEC `st`) THEN
 	    FULL_SIMP_TAC std_ss [FUNPOW, ARMCompositionTheory.get_st_def] THEN
 	    NTAC 2 (POP_ASSUM (K ALL_TAC)) THEN
-	    Induct_on `loopNum cond arm (\i.ARB) ((0,0w,st),{})` THENL [
+	    Induct_on `loopNum (translate_condition cond) arm (\i.ARB) ((0,0w,st),{})` THENL [
 	      REWRITE_TAC [Once EQ_SYM_EQ] THEN RW_TAC std_ss [FUNPOW,ARMCompositionTheory.get_st_def] THEN
 	      IMP_RES_TAC ARMCompositionTheory.LOOPNUM_BASIC THEN
 	      FULL_SIMP_TAC arith_ss [Once WHILE, ARMCompositionTheory.get_st_def],
 
 	    REWRITE_TAC [Once EQ_SYM_EQ] THEN RW_TAC std_ss [FUNPOW] THEN
-              IMP_RES_TAC ARMCompositionTheory.LOOPNUM_INDUCTIVE THEN
-	      `v = loopNum cond arm (\i.ARB) ((0,0w,SND (SND (FST (runTo (upload arm (\i.ARB) 0) (LENGTH arm) 
+        IMP_RES_TAC ARMCompositionTheory.LOOPNUM_INDUCTIVE THEN
+	      `v = loopNum (translate_condition cond) arm (\i.ARB) ((0,0w,SND (SND (FST (runTo (upload arm (\i.ARB) 0) (LENGTH arm) 
                    ((0,0w,st),{}))))),{})` by METIS_TAC [ABS_PAIR_THM,DECIDE (Term`!x.0+x=x`),
                        ARMCompositionTheory.LOOPNUM_INDEPENDENT_OF_CPSR_PCS, ARMCompositionTheory.get_st_def, 
                        FST, SND, ARMCompositionTheory.DSTATE_IRRELEVANT_PCS,ARMCompositionTheory.well_formed_def] THEN
@@ -383,14 +400,14 @@ val PRJ_TR_RULE = Q.store_thm (
 val PRJ_TR_RULE_2 = Q.store_thm (
    "PRJ_TR_RULE_2",
    `!cond ir stk_f cond_f prj_f f.
-        WELL_FORMED ir /\ (!st. cond_f (prj_f st) = eval_cond cond st) /\
+        WELL_FORMED ir /\ (!st. cond_f (prj_f st) = eval_il_cond cond st) /\
         (?R. WF R /\ !t0 t1. ~cond_f t0 ==> R (f t0) t0) /\
            PSPEC ir ((\st.T),(\st.T)) stk_f (prj_f,f,prj_f) ==> 
 		    PSPEC (TR cond ir) ((\st.T),(\st.T)) stk_f (prj_f, WHILE ($~ o cond_f) f, prj_f)`,
 
     SIMP_TAC std_ss [PSPEC_def, HSPEC_def] THEN
     REPEAT GEN_TAC THEN NTAC 2 STRIP_TAC THEN
-    `WF (\st1 st0. ~eval_cond cond st0 /\ (st1 = run_ir ir st0))` by METIS_TAC [WF_TR_LEM_2, WF_TR_LEM_3] THEN
+    `WF (\st1 st0. ~eval_il_cond cond st0 /\ (st1 = run_ir ir st0))` by METIS_TAC [WF_TR_LEM_2, WF_TR_LEM_3] THEN
     METIS_TAC [SIMP_RULE std_ss [PSPEC_def, HSPEC_def] (Q.SPECL [`cond`,`ir`,`\st.T`] PRJ_TR_RULE)]
   );
 
@@ -462,9 +479,10 @@ val _ = Hol_datatype `
          | VT of VEXP # VEXP         (* pairs     *)
     `;
 
-val readv_def = Define ` 
-    (readv st (PR (a,b)) = VT (readv st a, readv st b)) /\
-    (readv st x = SG (read st (toEXP x)))`;
+val readv_def = Define `
+     (readv st (PR (a,b)) = VT (readv st a, readv st b)) /\
+     (readv st x = SG (mread st x))`;
+
 
 (* Vector Stack, modelled as a list of expression vectors *)
 
@@ -511,7 +529,7 @@ val V_CJ_RULE = Q.store_thm (
    `!cond ir_t ir_f pre_p post_p stk cond_f iv f1 f2 ov. 
      WELL_FORMED ir_t /\ WELL_FORMED ir_f /\
      VSPEC ir_t (pre_p,post_p) stk (iv,f1,ov) /\ 
-     VSPEC ir_f (pre_p, post_p) stk (iv,f2,ov) /\ (!st. cond_f (readv st iv) = eval_cond cond st)
+     VSPEC ir_f (pre_p, post_p) stk (iv,f2,ov) /\ (!st. cond_f (readv st iv) = eval_il_cond cond st)
         ==>
        VSPEC (CJ cond ir_t ir_f) (pre_p,post_p) stk (iv, (\v.if cond_f v then f1 v else f2 v), ov)`,
      RW_TAC std_ss [VSPEC_def] THEN
@@ -523,8 +541,8 @@ val V_CJ_RULE = Q.store_thm (
 val V_TR_RULE = Q.store_thm (
    "V_TR_RULE",
    `!cond ir pre_p stk cond_f iv f.
-        WELL_FORMED ir /\  WF (\st1 st0. ~eval_cond cond st0 /\ (st1 = run_ir ir st0)) /\
-        (!st. cond_f (readv st iv) = eval_cond cond st) /\ VSPEC ir (pre_p,pre_p) stk (iv,f,iv) ==> 
+        WELL_FORMED ir /\  WF (\st1 st0. ~eval_il_cond cond st0 /\ (st1 = run_ir ir st0)) /\
+        (!st. cond_f (readv st iv) = eval_il_cond cond st) /\ VSPEC ir (pre_p,pre_p) stk (iv,f,iv) ==> 
           VSPEC (TR cond ir) (pre_p,pre_p) stk (iv, WHILE ($~ o cond_f) f, iv)`,
 
     RW_TAC std_ss [VSPEC_def] THEN 
@@ -583,6 +601,7 @@ val V_PUSH_RULE = Q.store_thm (
     METIS_TAC []
    );
 
+
 (*---------------------------------------------------------------------------------*)
 (*      Rules for Well-formedness                                                  *) 
 (*---------------------------------------------------------------------------------*)
@@ -590,11 +609,54 @@ val V_PUSH_RULE = Q.store_thm (
 val WELL_FORMED_TR_RULE = Q.store_thm (
    "WELL_FORMED_TR_RULE",
    `!cond ir context_f.
-        WELL_FORMED ir /\  WF (\st1 st0. ~eval_cond cond st0 /\ (st1 = run_ir ir st0)) ==>
+        WELL_FORMED ir /\  WF (\st1 st0. ~eval_il_cond cond st0 /\ (st1 = run_ir ir st0)) ==>
            WELL_FORMED (TR cond ir)`,
 
     RW_TAC std_ss [] THEN 
     METIS_TAC [IR_TR_IS_WELL_FORMED, WF_TR_LEM_1]
    );
+
+
+
+val IR_CJ_UNCHANGED = store_thm ("IR_CJ_UNCHANGED",
+``!cond ir_t ir_f s.
+	(WELL_FORMED ir_t /\ WELL_FORMED ir_f /\	
+	UNCHANGED s ir_t /\ UNCHANGED s ir_f)  ==>
+	UNCHANGED s (CJ cond ir_t ir_f)``,
+
+
+REWRITE_TAC[UNCHANGED_def] THEN 
+REPEAT STRIP_TAC THEN
+ASM_SIMP_TAC std_ss [SEMANTICS_OF_IR]  THEN
+PROVE_TAC[]);
+
+
+val IR_SC_UNCHANGED = store_thm ("IR_SC_UNCHANGED",
+``!ir1 ir2 s.
+	(WELL_FORMED ir1 /\ WELL_FORMED ir2 /\	
+	UNCHANGED s ir1 /\ UNCHANGED s ir2)  ==>
+	UNCHANGED s (SC ir1 ir2)``,
+
+
+REWRITE_TAC[UNCHANGED_def] THEN 
+REPEAT STRIP_TAC THEN
+ASM_SIMP_TAC std_ss [SEMANTICS_OF_IR]  THEN
+PROVE_TAC[])
+
+val UNCHANGED_TR_RULE = store_thm ("UNCHANGED_TR_RULE",
+``!c ir s.
+	(WELL_FORMED (TR c ir) /\ UNCHANGED s ir) ==>
+	UNCHANGED s (TR c ir)``,
+
+  REWRITE_TAC [UNCHANGED_def, WELL_FORMED_def] THEN
+  REPEAT STRIP_TAC THEN
+  ASM_SIMP_TAC std_ss [IR_SEMANTICS_TR___FUNPOW] THEN
+  Q.ABBREV_TAC `n = (shortest (eval_il_cond c) (run_ir ir) st)` THEN
+  POP_ASSUM (fn x => ALL_TAC) THEN
+  Induct_on `n` THENL [
+	 REWRITE_TAC[FUNPOW],
+	 REWRITE_TAC[FUNPOW_SUC] THEN PROVE_TAC[]
+  ]);
+		
 
 val _ = export_theory();
